working on freshness

src/FcEtt/ett_path.v
@@ -88,6 +88,42 @@ Proof. intros. pose (P := CasePath_binds_toplevel H).
        pose (Q3 := match_dec). pose (Q4 := Q3 a p (CasePath_lc H)).
        inversion Q4; eauto.
 Qed.
+
+Fixpoint var_patt (p : tm) : atoms := 
+   match p with
+      a_App p (Role R) (a_Var_f x) => (singleton x) \u (var_patt p)
+    | a_App p (Rho Irrel) Bullet => var_patt p
+    | a_CApp p g_Triv => var_patt p
+    | _  => {}
+   end.
+
+Lemma MatchSubst_subst : forall a p b1 x y b2,
+     MatchSubst a p (tm_subst_tm_tm (a_Var_f y) x b1) b2 ->
+     y `notin` fv_tm_tm_tm a -> y `notin` var_patt(p) -> x `notin` var_patt(p) ->
+     MatchSubst a p b1 (tm_subst_tm_tm (a_Var_f x) y b2).
+Proof. intros. dependent induction H.
+        - admit.
+        - simpl in *. eapply MatchSubst_AppRelR in IHMatchSubst; eauto 2.
+          erewrite tm_subst_tm_tm_tm_subst_tm_tm in IHMatchSubst; eauto 2.
+          assert (a_Var_f x = tm_subst_tm_tm a x0 (a_Var_f x)).
+          simpl. destruct (x == x0); eauto. apply notin_union_1 in H3.
+          apply notin_singleton_1 in H3. symmetry in e. contradiction.
+          rewrite H4. eauto.
+        - simpl in *. eauto.
+        - simpl in *. eauto.
+Admitted.
+
+Lemma MatchSubst_Rename : forall p1 p2 a1 a2 W a b, Rename p1 a1 p2 a2 W ->
+                                 MatchSubst a p1 a1 b ->
+                                 MatchSubst a p2 a2 b.
+Proof. intros. generalize dependent p2. generalize dependent a2.
+       generalize dependent W. induction H0; intros.
+        - inversion H0; subst. eauto.
+        - inversion H1; subst. apply IHMatchSubst in H9.
+          eapply MatchSubst_AppRelR in H9; auto. admit.
+        - inversion H; subst. eauto.
+        - inversion H; subst. eauto.
+Admitted.
 (*
 Lemma subst_CasePath : forall F a b R x, lc_tm b -> Value R a ->
                    CasePath R (tm_subst_tm_tm b x a) F -> CasePath R a F.
